Sorting/MergeSort.v
@@ -12,8 +12,9 @@ Require Import InsertionSort.
 Set Implicit Arguments.
 
 Function merge (A : LinDec) (l : list A * list A)
-    {measure lenSum l} : list A :=
-let (l1, l2) := l in match l1, l2 with
+  {measure lenSum l} : list A :=
+  let (l1, l2) := l in
+match l1, l2 with
     | [], _ => l2
     | _, [] => l1
     | h :: t, h' :: t' =>
@@ -26,78 +27,45 @@ Proof.
   intros. unfold lenSum. simpl. omega.
 Defined.
 
-Hint Extern 1 (length (drop _ _) < length _) =>
-  apply drop_length_lt; simpl; [omega | inversion 1].
-
-Hint Extern 1 (length (take _ _) < length _) =>
-  apply take_length_lt; apply lt_div2; simpl; omega.
-
-Function ms (A : LinDec) (l : list A) {measure length l} : list A :=
-match l with
-    | [] => []
-    | [x] => [x]
-    | l' =>
-      let n := div2 (length l') in
-      let l1 := take n l' in
-      let l2 := drop n l' in
-      merge A (ms A l1, ms A l2)
-end.
-Proof. all: auto. Defined.
-
-Hint Extern 1 (length _ < length _) =>
-match goal with
-    | H : context [ms_split] |- _ =>
-        try (eapply ms_split_len1; eauto; fail);
-        eapply ms_split_len2; eauto
-end.
-
-Function ms2 (A : LinDec) (l : list A) {measure length l} : list A :=
-match l with
-    | [] => []
-    | [x] => [x]
-    | l' =>
-        let (l1, l2) := ms_split l' in
-          merge A (ms2 A l1, ms2 A l2)
-end.
-Proof. all: auto. Defined.
-
-Hint Extern 1 (length _ < length _) =>
-match goal with
-    | H : (length ?l <=? S (S _)) = false |- _ =>
-        destruct l as [| ? | ? ? ?] using list_ind2;
-        simpl in H; inversion_clear H
-end.
-
-Function hms (n : nat) (A : LinDec) (sort : list A -> list A) (l : list A)
-  {measure length l} : list A :=
-  if @leqb natle (length l) (S (S n))
-  then sort l
-  else  let n := Nat.div2 (length l) in
-        let l1 := take n l in
-        let l2 := drop n l in
-          merge A (hms n A sort l1, hms n A sort l2).
+Theorem merge_sorted :
+  forall (A : LinDec) (l : list A * list A),
+    sorted A (fst l) -> sorted A (snd l) -> sorted A (merge A l).
 Proof.
-  all: auto.
-Defined. 
+  intros. functional induction merge A l; simpl in *; auto;
+  rewrite merge_equation in *.
+    destruct t; simpl in *; dec.
+    destruct t'; simpl in *; dec.
+Qed.
 
-(* Parametrized mergesort *)
-Function hms2 (n : nat) (A : LinDec) (sort : list A -> list A) (l : list A)
-  {measure length l} : list A :=
-  if @leqb natle (length l) (S (S n))
-  then sort l
-  else let (l1, l2) := ms_split l in
-    merge A (hms2 n A sort l1, hms2 n A sort l2).
+Theorem merge_perm :
+  forall (A : LinDec) (l : list A * list A),
+    perm A (fst l ++ snd l) (merge A l).
 Proof.
-  all: auto.
-Defined.
+  intros. functional induction merge A l; simpl; auto; try clear y.
+    rewrite app_nil_r. auto.
+    eapply perm_trans.
+      rewrite app_comm_cons. apply perm_app_comm.
+      simpl. apply perm_cons. simpl in IHl0. rewrite <- IHl0.
+        apply perm_app_comm.
+Qed.
 
-Class Split (A : Type) : Type :=
+Theorem merge_pres_perm :
+  forall (A : LinDec) (l1 l1' l2 l2' : list A),
+    perm A l1 l1' -> perm A l2 l2' ->
+      perm A (merge A (l1, l2)) (merge A (l1', l2')).
+Proof.
+  intros. rewrite <- !merge_perm. cbn. apply perm_app; assumption.
+Qed.
+
+Class Split (A : LinDec) : Type :=
 {
     split' : list A -> list A * list A;
-    spec1 : forall l l1 l2 : list A,
+    split'_spec1 : forall l l1 l2 : list A,
         split' l = (l1, l2) -> 2 <= length l -> length l1 < length l;
-    spec2 : forall l l1 l2 : list A,
+    split'_spec2 : forall l l1 l2 : list A,
         split' l = (l1, l2) -> 2 <= length l -> length l2 < length l;
+    perm_split_app : forall (l : list A),
+        perm A l (fst (split' l) ++ snd (split' l))
 }.
 
 Coercion split' : Split >-> Funclass.
@@ -105,26 +73,86 @@ Coercion split' : Split >-> Funclass.
 Function ghms (n : nat) (A : LinDec)
   (sort : list A -> list A) (split : Split A)
   (l : list A) {measure length l} : list A :=
-    if @leqb natle (length l) (S (S n))
+    if @leqb natle (length l) (S n)
     then sort l
     else let (l1, l2) := split l in
-      merge A (ghms n A sort split l1, ghms n A sort split l2).
+      merge A (@ghms n A sort split l1, @ghms n A sort split l2).
 Proof.
-  intros. apply spec2 with l1.
-    assumption.
-    destruct (@leqb_spec natle (length l) (S (S n))); cbn in *.
-      congruence.
-      omega.
-  intros. apply spec1 with l2.
-    assumption.
-    destruct (@leqb_spec natle (length l) (S (S n))); cbn in *.
-      congruence.
-      omega.
+  intros. apply split'_spec2 with l1; dec.
+    dec. cbn in *. omega.
+  intros. apply split'_spec1 with l2; dec.
+    dec. cbn in *. omega.
 Defined.
+
+Lemma div2_lt_S :
+  forall n : nat, div2 n < S n.
+Proof.
+  intros. functional induction @div2 n; omega.
+Qed.
+
+Instance HalfSplit (A : LinDec) : Split A :=
+{
+    split' l :=
+      let n := div2 (length l) in
+      let l1 := take n l in
+      let l2 := drop n l in (l1, l2)
+}.
+Proof.
+  intros. destruct l as [| x [| y t]]; cbn in *.
+    omega.
+    omega.
+    inversion H; subst; cbn. apply lt_n_S. apply take_length_lt. cbn.
+      apply div2_lt_S.
+  intros. inversion H; subst. apply drop_length_lt. cbn.
+    destruct l as [| x [| y t]]; cbn in *; omega.
+    destruct l as [| x [| y t]]; cbn in *; inversion 1. omega.
+  intros. cbn. rewrite take_drop. reflexivity.
+Defined.
+
+Fixpoint interleave {A : Type} (l1 l2 : list A) : list A :=
+match l1, l2 with
+    | [], _ => l2
+    | _, [] => l1
+    | h1 :: t1, h2 :: t2 => h1 :: h2 :: interleave t1 t2
+end.
+
+Theorem ms_split_interleave :
+  forall (A : Type) (l : list A),
+    interleave (fst (ms_split l)) (snd (ms_split l)) = l.
+Proof.
+  induction l as [| | h h' t] using list_ind2; cbn; auto.
+    destruct (ms_split t). cbn in *. rewrite IHt. auto.
+Qed.
+
+Lemma count_interleave :
+  forall (A : LinDec) (x : A) (l1 l2 : list A),
+    count A x (interleave l1 l2) = count A x l1 + count A x l2.
+Proof.
+  induction l1 as [| h1 t1]; cbn; auto.
+    destruct l2 as [| h2 t2]; cbn.
+      apply plus_n_O.
+      dec; rewrite IHt1; omega.
+Qed.
+
+Lemma perm_interleave :
+  forall (A : LinDec) (l1 l1' l2 l2' : list A),
+    perm A l1 l1' -> perm A l2 l2' ->
+      perm A (interleave l1 l2) (interleave l1' l2').
+Proof.
+  unfold perm. intros. rewrite !count_interleave. auto.
+Qed.
+
+Lemma merge_perm_interleave :
+  forall (A : LinDec) (l : list A * list A),
+    perm A (merge A l) (interleave (fst l) (snd l)).
+Proof.
+  unfold perm; intros. rewrite count_interleave.
+  rewrite <- merge_perm. rewrite count_app. auto.
+Qed.
 
 Instance MsSplit (A : LinDec) : Split A :=
 {
-    split' := ms_split
+    split' := ms_split;
 }.
 Proof.
   intros. destruct l as [| x [| y t]]; cbn in *.
@@ -135,9 +163,15 @@ Proof.
     omega.
     omega.
     eapply ms_split_len2. eauto.
+  intros. rewrite <- ms_split_interleave at 1.
+    rewrite <- merge_perm_interleave. rewrite merge_perm. reflexivity.
 Defined.
 
-Definition wut (A : LinDec) (l : list A) : list A :=
-  ghms 0 A (fun l => l) (MsSplit A) l.
+Definition ms (A : LinDec) :=
+  @ghms 0 A (fun l => l) (MsSplit A).
 
-Compute wut natle testl.
+Definition ms2 (A : LinDec) :=
+  @ghms 0 A (fun l => l) (HalfSplit A).
+
+Compute ms natle testl.
+Compute ms2 natle testl.
