Sorting/MergeSortSpec.v
@@ -5,188 +5,23 @@ Require Import InsertionSort.
 
 Set Implicit Arguments.
 
-Theorem merge_sorted :
-  forall (A : LinDec) (l : list A * list A),
-    sorted A (fst l) -> sorted A (snd l) -> sorted A (merge A l).
+Theorem ghms_sorted :
+  forall (n : nat) (A : LinDec)
+    (s : Sort) (split : Split A)
+      (l : list A), sorted A (@ghms n A (@sort s A) split l).
 Proof.
-  intros. functional induction merge A l; simpl in *; auto;
-  rewrite merge_equation in *.
-    destruct t; simpl in *; dec.
-    destruct t'; simpl in *; dec.
+  intros. functional induction @ghms n A (@sort s A) split l.
+    destruct s; cbn in *. apply sort_sorted.
+    apply merge_sorted; cbn; assumption.
 Qed.
 
-Theorem merge_perm :
-  forall (A : LinDec) (l : list A * list A),
-    perm A (fst l ++ snd l) (merge A l).
+Theorem ghms_perm :
+  forall (n : nat) (A : LinDec)
+    (s : Sort) (split : Split A)
+      (l : list A), perm A l (@ghms n A (@sort s A) split l).
 Proof.
-  intros. functional induction merge A l; simpl; auto; try clear y.
-    rewrite app_nil_r. auto.
-    eapply perm_trans.
-      rewrite app_comm_cons. apply perm_app_comm.
-      simpl. apply perm_cons. simpl in IHl0. rewrite <- IHl0.
-        apply perm_app_comm.
+  intros. functional induction @ghms n A (@sort s A) split l.
+    destruct s; cbn in *. apply sort_perm.
+    rewrite perm_split_app. rewrite e0; cbn.
+      rewrite <- merge_perm; cbn. apply perm_app; assumption.
 Qed.
-
-Theorem ms_sorted :
-  forall (A : LinDec) (l : list A), sorted A (ms A l).
-Proof.
-  intros. functional induction ms A l; auto; clear y.
-  apply merge_sorted; simpl; assumption.
-Qed.
-
-Theorem ms_perm :
-  forall (A : LinDec) (l : list A), perm A l (ms A l).
-Proof.
-  intros. functional induction ms A l; auto; clear y.
-  rewrite <- merge_perm, <- (take_drop (Nat.div2 (length l))) at 1; simpl.
-  apply perm_app; assumption.
-Qed.
-
-Instance Sort_ms : Sort :=
-{
-    sort := ms;
-    sort_sorted := ms_sorted;
-    sort_perm := ms_perm;
-}.
-
-(* Specification of ms2. *)
-Theorem ms2_sorted :
-  forall (A : LinDec) (l : list A), sorted A (ms2 A l).
-Proof.
-  intros. functional induction ms2 A l; auto; clear y.
-  apply merge_sorted; simpl; assumption.
-Qed.
-
-Fixpoint interleave {A : Type} (l1 l2 : list A) : list A :=
-match l1, l2 with
-    | [], _ => l2
-    | _, [] => l1
-    | h1 :: t1, h2 :: t2 => h1 :: h2 :: interleave t1 t2
-end.
-
-Theorem ms_split_interleave :
-  forall (A : Type) (l : list A),
-    interleave (fst (ms_split l)) (snd (ms_split l)) = l.
-Proof.
-  induction l as [| | h h' t] using list_ind2; cbn; auto.
-    destruct (ms_split t). cbn in *. rewrite IHt. auto.
-Qed.
-
-Theorem interleave_ms_split :
-  forall (A : Type) (l1 l2 : list A),
-    ms_split (interleave l1 l2) = (l1, l2).
-Proof.
-  induction l1 as [| h1 t1]. cbn.
-Abort.
-
-Lemma count_interleave :
-  forall (A : LinDec) (x : A) (l1 l2 : list A),
-    count A x (interleave l1 l2) = count A x l1 + count A x l2.
-Proof.
-  induction l1 as [| h1 t1]; cbn; auto.
-    destruct l2 as [| h2 t2]; cbn.
-      apply plus_n_O.
-      dec; rewrite IHt1; omega.
-Qed.
-
-Lemma perm_interleave :
-  forall (A : LinDec) (l1 l1' l2 l2' : list A),
-    perm A l1 l1' -> perm A l2 l2' ->
-      perm A (interleave l1 l2) (interleave l1' l2').
-Proof.
-  unfold perm. intros. rewrite !count_interleave. auto.
-Qed.
-
-Lemma merge_perm_interleave :
-  forall (A : LinDec) (l : list A * list A),
-    perm A (merge A l) (interleave (fst l) (snd l)).
-Proof.
-  unfold perm; intros. rewrite count_interleave.
-  rewrite <- merge_perm. rewrite count_app. auto.
-Qed.
-
-Theorem ms2_perm :
-  forall (A : LinDec) (l : list A), perm A l (ms2 A l).
-Proof.
-  intros. functional induction ms2 A l; auto; clear y.
-  rewrite merge_perm_interleave. simpl.
-    rewrite <- ms_split_interleave at 1. apply perm_interleave.
-      rewrite e0. simpl. auto.
-      rewrite e0. simpl. auto.
-Qed.
-
-Instance Sort_ms2 : Sort :=
-{
-    sort := ms2;
-    sort_sorted := ms2_sorted;
-    sort_perm := ms2_perm;
-}.
-
-(* Specification of hms. *)
-Theorem hms_sorted :
-  forall (n : nat) (A : LinDec) (sort : list A -> list A)
-    (sort_perm : forall l : list A, perm A l (sort l))
-    (sort_sorted : forall l : list A, sorted A (sort l))
-      (l : list A), sorted A (hms n A sort l).
-Proof.
-  intros. functional induction hms n A sort l; auto.
-    apply merge_sorted; cbn; auto.
-Qed.
-
-Theorem hms_perm :
-  forall (n : nat) (A : LinDec) (sort : list A -> list A)
-    (sort_perm : forall l : list A, perm A l (sort l))
-    (sort_sorted : forall l : list A, sorted A (sort l))
-      (l : list A), perm A l (hms n A sort l).
-Proof.
-  intros. functional induction hms n A sort l; auto.
-    rewrite <- merge_perm, <- (take_drop (Nat.div2 (length l))) at 1; simpl.
-      apply perm_app; auto.
-Qed.
-
-(*Instance Sort_hms (n : nat) : Sort :=
-{
-    sort := hms n;
-    sort_sorted := hms_sorted n;
-    sort_perm := hms_perm n;
-}.*)
-
-(* TODO *) Lemma ms2_is_ms :
-  forall (A : LinDec) (l : list A), ms2 A l = ms A l.
-Proof.
-  intros. functional induction ms2 A l; auto.
-    rewrite ms_equation. destruct l as [| h [| h' t]]; inversion y.
-      rewrite IHl0, IHl1.
-Abort.
-
-(* Specification of hms3. *)
-Theorem hms2_sorted :
-  forall (n : nat) (A : LinDec) (sort : list A -> list A)
-    (sort_perm : forall l : list A, perm A l (sort l))
-    (sort_sorted : forall l : list A, sorted A (sort l))
-      (l : list A), sorted A (hms2 n A sort l).
-Proof.
-  intros. functional induction hms2 n A sort l; auto.
-    apply merge_sorted; simpl; assumption.
-Qed.
-
-Theorem hms2_perm :
-  forall (n : nat) (A : LinDec) (sort : list A -> list A)
-    (sort_perm : forall l : list A, perm A l (sort l))
-    (sort_sorted : forall l : list A, sorted A (sort l))
-      (l : list A), perm A l (hms2 n A sort l).
-Proof.
-  intros. functional induction hms2 n A sort l; auto.
-    rewrite merge_perm_interleave. simpl.
-      rewrite <- ms_split_interleave at 1. apply perm_interleave.
-        rewrite e0. simpl. auto.
-        rewrite e0. simpl. auto.
-Qed.
-
-(* TODO *)
-(*Instance Sort_hms3 (n : nat) : Sort :=
-{
-    sort := hms3 n;
-    sort_sorted := hms2_sorted n;
-    sort_perm := hms2_perm n;
-}.*)
