Sorting/Test.v
@@ -51,3 +51,32 @@ Time Compute leftistHeapsort natle (cycle 20 testl).
 Time Compute hqs 1024 natle (cycle 2000 [1]).
 Time Compute hms 1024 natle (cycle 2000 [1]).
 Time Compute treeSort natle (cycle 2000 [1]).*)
+
+(*Time Compute ms natle (cycle 3000 wut).
+Time Compute qs natle (cycle 3000 wut).*)
+
+Require Import TrichQuicksort.
+Require Import TrichDec.
+
+Definition wut := [1].
+
+Time Compute tqs natlt (cycle 3000 wut).
+
+Fixpoint toN (n : nat) : list nat :=
+match n with
+    | 0 => [0]
+    | S n' => n :: toN n'
+end.
+
+(*CoFixpoint rand (seed n1 n2 : Z) : Stream Z :=
+let seed' := Zmod seed n2 in Cons seed' (rand (seed' * n1) n1 n2).*)
+
+Require Import RedBlack.
+
+Time Compute qs natle (toN 200).
+Time Compute tqs natlt (toN 200).
+Time Compute insertionSort natle (toN 150).
+Time Compute redblackSort natle (toN 150).
+
+Time Compute htqs 1024 natlt (insertionSort natle) (cycle 500 testl).
+Time Compute htqs 256 natlt (redblackSort natle) (cycle 500 testl).
