Trees/RedBlack.v
@@ -1,0 +1,406 @@
+Add Rec LoadPath "/home/zeimer/Code/Coq".
+
+Require Import BTree.
+Require Export LinDec.
+Require Import Sorting.Sort.
+
+Inductive color : Set :=
+    | Red : color
+    | Black : color.
+
+Inductive RBTree (A : Type) : Type :=
+    | E : RBTree A
+    | T : color -> RBTree A -> A -> RBTree A -> RBTree A.
+
+Arguments E [A].
+Arguments T [A] _ _ _.
+
+Inductive elem {A : Type} (x : A) : RBTree A -> Prop :=
+    | elem_root : forall (c : color) (l r : RBTree A),
+        elem x (T c l x r)
+    | elem_left : forall (c : color) (v : A) (l r : RBTree A),
+        elem x l -> elem x (T c l v r)
+    | elem_right : forall  (c : color) (v : A) (l r : RBTree A),
+        elem x r -> elem x (T c l v r).
+
+Hint Constructors color RBTree elem.
+
+Ltac inv H := inversion H; clear H; subst; cbn; auto.
+
+Lemma elem_color :
+  forall (A : Type) (c c' : color) (x v : A) (l r : RBTree A),
+    elem x (T c l v r) -> elem x (T c' l v r).
+Proof.
+  intros; inv H.
+Qed.
+
+Function balance {A : Type} (c : color)
+  (l : RBTree A) (v : A) (r : RBTree A) : RBTree A :=
+match c with
+    | Red => T Red l v r
+    | Black =>
+        match l, v, r with
+            | T Red (T Red a xv b) yv c, zv, d
+            | T Red a xv (T Red b yv c), zv, d
+            | a, xv, T Red (T Red b yv c) zv d
+            | a, xv, T Red b yv (T Red c zv d) =>
+                T Red (T Black a xv b) yv (T Black c zv d)
+            | l, v, r => T Black l v r
+        end
+end.
+
+Definition makeBlack {A : Type} (t : RBTree A) :=
+match t with
+    | E => E
+    | T _ l v r => T Black l v r
+end.
+
+(*Function ins {A : LinDec} (x : A) (t : RBTree A) : RBTree A :=
+match t with
+    | E => T Red E x E
+    | T c l v r =>
+        if x <=? v
+        then balance c (ins x l) v r
+        else if v <=? x
+          then balance c l v (ins x r)
+          else T c l x r
+end.*)
+
+Function ins {A : LinDec} (x : A) (t : RBTree A) : RBTree A :=
+match t with
+    | E => T Red E x E
+    | T c l v r =>
+        if x <=? v
+        then balance c (ins x l) v r
+        else balance c l v (ins x r)
+end.
+
+Definition insert {A : LinDec} (x : A) (t : RBTree A) : RBTree A :=
+  makeBlack (ins x t).
+
+Require Import Coq.Logic.FunctionalExtensionality.
+
+Lemma T_not_E :
+  forall (A : Type) (c : color) (v : A) (l r : RBTree A),
+    T c l v r <> E.
+Proof.
+  inversion 1.
+Qed.
+
+Lemma balance_not_E :
+  forall (A : Type) (c : color) (v : A) (l r : RBTree A),
+    balance c l v r <> E.
+Proof.
+  intros. functional induction @balance A c l v r; apply T_not_E.
+Qed.
+
+Lemma balance_is_T :
+  forall (A : Type) (c : color) (v : A) (l r : RBTree A),
+    exists (c' : color) (v' : A) (l' r' : RBTree A),
+      balance c l v r = T c' l' v' r'.
+Proof.
+  intros. functional induction @balance A c l v r; eauto 6.
+Qed.
+
+(*Ltac dst := repeat
+match goal with
+    | |- context [if ?x then _ else _] => destruct x
+    | |- context [match ?x with _ => _ end] => destruct x
+end; try apply T_not_E.*)
+
+Lemma ins_not_E :
+  forall (A : LinDec) (x : A) (t : RBTree A),
+    ins x t <> E.
+Proof.
+  intros. functional induction @ins A x t;
+  try apply T_not_E; apply balance_not_E.
+Qed.
+
+Inductive is_bst {A : LinDec} : RBTree A -> Prop :=
+    | is_bst_E : is_bst E
+    | is_bst_T : forall (c : color) (v : A) (l r : RBTree A),
+        (forall x : A, elem x l -> leq x v) -> is_bst l ->
+        (forall x : A, elem x r -> leq v x) -> is_bst r ->
+        is_bst (T c l v r).
+
+Hint Constructors is_bst.
+
+Lemma color_is_bst :
+  forall (A : LinDec) (c c' : color) (v : A) (l r : RBTree A),
+    is_bst (T c l v r) <-> is_bst (T c' l v r).
+Proof.
+  split; intros; inv H.
+Qed.
+
+Hint Resolve elem_color.
+
+(*Lemma balance_is_bst :
+  forall (A : LinDec) (c : color) (v : A) (l r : RBTree A),
+    is_bst (T c l v r) -> is_bst (balance c l v r).
+Proof.
+  intros. functional induction @balance (@carrier A) c l v r;
+  try assumption.
+    inv H. inv H5. inv H8. constructor; intros; auto.
+      apply H3. eapply elem_color. eauto.
+      inv H.
+      apply H3.
+      apply *)
+
+(*Ltac bd := intros; repeat (match goal with
+    | |- context [if ?x then _ else _] =>
+        bdestruct (x); subst; cbn in *; try discriminate; auto
+    | H : (?x <? ?y) = _ |- _ => destruct (blt_reflect x y); try congruence
+    | H : ?x <> ?x |- _ => contradiction
+    | H : ?x = ?x |- _ => clear H
+    | H : ~ ?x < ?y, H' : ~ ?y < ?x |- _ =>
+        assert (x = y) by (unfold key in *; omega); subst; clear H; clear H'
+    | H : Abs E _ |- _ => inv H    
+    | H : Abs (T _ _ _ _ _) _ |- _ => inv H
+    | _ => auto; omega
+end; st; cbn in *)
+
+Ltac ext x := extensionality x.
+
+Fixpoint toList' {A : Type} (t : RBTree A) (acc : list A) : list A :=
+match t with
+    | E => acc
+    | T _ l v r => toList' l (v :: toList' r acc)
+end.
+
+Definition toList {A : Type} (t : RBTree A) : list A := toList' t [].
+
+Function slow_toList {A : Type} (t : RBTree A) : list A :=
+match t with
+    | E => []
+    | T _ l v r => slow_toList l ++ v :: slow_toList r
+end.
+
+Lemma aux :
+  forall (A : Type) (t : RBTree A) (acc : list A),
+    toList' t acc = slow_toList t ++ acc.
+Proof.
+  induction t; cbn; intros.
+    trivial.
+    rewrite IHt1, IHt2, <- app_assoc, <- app_comm_cons. trivial.
+Qed.
+
+Theorem toList_is_slow: @toList = @slow_toList.
+Proof.
+  ext A. ext t. unfold toList. rewrite aux. rewrite app_nil_r. trivial.
+Qed.
+
+Ltac gen H := generalize dependent H.
+
+Fixpoint fromList {A : LinDec} (l : list A) : RBTree A :=
+match l with
+    | [] => E
+    | h :: t => ins h (fromList t)
+end.
+
+Print fold_left.
+
+Definition fromList' {A : LinDec} (l : list A) : RBTree A :=
+  fold_left (fun t x => ins x t) l E.
+
+Definition redblackSort (A : LinDec) (l : list A) : list A :=
+  toList (fromList l).
+
+Definition redblackSort' (A : LinDec) (l : list A) : list A :=
+  toList (fromList' l).
+
+Definition redblackSort'' (A : LinDec) (l : list A) : list A :=
+  slow_toList (fromList' l).
+
+
+Require Import ListLemmas.
+
+Time Compute redblackSort natle (cycle 200 testl).
+Time Compute redblackSort' natle (cycle 200 testl).
+Time Compute redblackSort'' natle (cycle 200 testl).
+
+(*
+Lemma list2map_app_left :
+  forall (al bl : list (key * V)) (i : key) v,
+    In (i, v) al -> list2map (al ++ bl) (int2Z i) = list2map al (int2Z i).
+Proof.
+  induction al as [| h t]; cbn; intros; inv H.
+    rewrite !t_update_eq. trivial.
+    destruct h. destruct (Z.eq_dec (int2Z k) (int2Z i)).
+      rewrite e. rewrite !t_update_eq. trivial.
+      rewrite !t_update_neq; try inversion 1; auto. eauto.
+Qed.
+
+Lemma list2map_app_right :
+  forall (al bl : list (key * V)) (i : Z),
+    ~ (exists k v, int2Z k = i /\ In (k, v) al) ->
+      list2map (al ++ bl) i = list2map bl i.
+Proof.
+  induction al as [| h t]; cbn; intros.
+    trivial.
+    destruct h. destruct (Z.eq_dec (int2Z k) i).
+      subst. contradiction H. eauto.
+      rewrite t_update_neq; auto.
+        apply IHt. contradict H. decompose [ex and] H. eauto.
+Qed.
+
+Lemma list2map_app_not_in_default :
+  forall (al : list (key * V)) (i : Z),
+    ~ (exists k v, int2Z k = i /\ In (k, v) al) ->
+      list2map al i = default.
+Proof.
+  induction al as [| h t]; cbn; intros.
+    compute. trivial.
+    destruct h. destruct (Z.eq_dec (int2Z k) i).
+      subst. contradiction H. eauto.
+      rewrite t_update_neq; auto.
+        apply IHt. contradict H. decompose [ex and] H. eauto.
+Qed.
+
+Lemma no_elem_nil :
+  forall (A : Type) (l : list A),
+    ~ (exists x : A, In x l) -> l = [].
+Proof.
+  induction l as [| h t]; cbn; intro.
+    trivial.
+    cut False; [inversion 1 |]. apply H. eauto.
+Qed.
+
+Lemma no_elem_nil' :
+  forall l : list (key * V),
+    (forall k : key, ~ (exists v : V, In (k, v) l)) -> l = [].
+Proof.
+  intros. apply no_elem_nil. intro. destruct H0 as [[k v] H'].
+  specialize (H k). firstorder.
+Qed.
+
+Theorem elements_relate :
+  forall t m,
+    SearchTree t -> Abs t m -> list2map (elements t) = m.
+Proof.
+  rewrite elements_slow_elements.
+  intros until 1. inv H. gen m.
+  induction H0; intros; bd.
+  specialize (IHSearchTree'1 _ H6); clear H6.
+  specialize (IHSearchTree'2 _ H7); clear H7.
+  ext k'.
+  destruct (In_decidable (slow_elements l) k') as [[k'' [v' [Heq Hin]]] |].
+    rewrite <- Heq, list2map_app_left with (v := v'); auto. subst.
+      assert (H' := slow_elements_range _ _ _ _ _ H0_ Hin).
+      unfold t_update, combine; cbn. bd.
+    destruct (In_decidable (slow_elements r) k') as [[k'' [v' [Heq Hin]]] |].
+      rewrite -> list2map_app_right; auto.
+        assert (H'' := slow_elements_range _ _ _ _ _ H0_0 Hin).
+        unfold t_update, combine; subst; cbn. bd. rewrite t_update_neq; auto.
+      subst.
+        rewrite -> list2map_app_right; auto; cbn.
+        apply list2map_app_not_in_default in H.
+        apply list2map_app_not_in_default in H0.
+        unfold t_update, combine; cbn. bd.
+        destruct (Z_ltb_reflect k' (int2Z k)); bd.
+Qed.
+
+(* Ex. is_redblack *)
+Inductive is_redblack : RBTree -> color -> nat -> Prop :=
+    | IsRB_leaf : forall c, is_redblack E c 0
+    | IsRB_r : forall l k v r n,
+        is_redblack l Red n -> is_redblack r Red n ->
+        is_redblack (T Red l k v r) Black n
+    | IsRB_b : forall c l k v r n,
+        is_redblack l Black n -> is_redblack r Black n ->
+        is_redblack (T Black l k v r) c (S n).
+
+Hint Constructors is_redblack.
+
+Lemma is_redblack_toblack :
+  forall t n, is_redblack t Red n -> is_redblack t Black n.
+Proof.
+  induction 1; eauto.
+Qed.
+
+Hint Resolve is_redblack_toblack.
+
+Inductive nearly_redblack : RBTree -> nat -> Prop :=
+    | nrRB_r : forall l k v r n,
+        is_redblack l Black n -> is_redblack r Black n ->
+        nearly_redblack (T Red l k v r) n
+    | nrRB_b : forall l k v r n,
+        is_redblack l Black n -> is_redblack r Black n ->
+        nearly_redblack (T Black l k v r) (S n).
+
+Hint Constructors nearly_redblack.
+
+Ltac irb := repeat
+match goal with
+    | H : is_redblack E _ _ |- _ => inv H
+    | H : is_redblack (T _ _ _ _ _) _ _ |- _ => inv H
+(*    | H : is_redblack (T _ _ _ _ _) _ (S _) |- _ => inv H*)
+    | H : nearly_redblack E _ |- _ => inv H
+    | H : nearly_redblack (T _ _ _ _ _) _ |- _ => inv H
+end.
+
+Lemma ins_is_redblack :
+  forall k v t n,
+    (is_redblack t Black n -> nearly_redblack (ins k v t) n) /\
+    (is_redblack t Red n -> is_redblack (ins k v t) Black n).
+Proof.
+  Time induction t; cbn; split; intros; irb; bd;
+  repeat match goal with
+      | n : nat, IH : forall _ : nat, _ |- _ =>
+          decompose [and] (IH n); clear IH
+      | x : ?A, f : ?A -> _ |- _ => specialize (f x)
+  end;
+  dst; irb; st; repeat constructor; auto.
+Qed.
+
+Lemma insert_is_redblack :
+  forall k v t n, is_redblack t Red n ->
+    exists n', is_redblack (insert k v t) Red n'.
+Proof.
+  unfold insert.
+  intros k v t. functional induction (ins k v t); cbn; intros; irb; st.
+    exists 1%nat. eauto.
+    decompose [ex] (balance_is_T Black (ins k v l) k0 v0 r).
+      rewrite H. cbn. exists (S n0). econstructor. eauto.
+
+Restart.
+Ltac omg := repeat (cbn in *; match goal with
+    | H : is_redblack E _ _ |- _ => inv H
+    | H : is_redblack _ _ 0 |- _ => inv H
+    | H : is_redblack (T _ _ _ _ _) _ _ |- _ => inv H
+    | |- context [ltb ?x ?y] =>
+        destruct (int_blt_reflect x y); try congruence
+    | H : context [ltb ?x ?y] |- _ =>
+        destruct (int_blt_reflect x y); try congruence; clear H
+    | |- context [match (ins ?k ?v ?t) with _ => _ end] =>
+        case_eq (ins k v t); intros
+    | H : context [match (ins ?k ?v ?t) with _ => _ end] |- _ =>
+        case_eq (ins k v t); intros
+    | H : ins _ _ _ = E |- _ => apply ins_not_E in H; inv H
+    | H : ins ?k ?v ?t = _, H' : context [ins ?k ?v ?t] |- _ =>
+        rewrite H in H'
+    | |- context [match ?x with _ => _ end] => destruct x
+    | c : color |- _ => destruct c
+    | H : context [match ?x with _ => _ end] |- _ => destruct x
+    | H : ~ ?x < ?y, H' : ~ ?y < ?x |- _ =>
+        assert (x = y) by (unfold key in *; omega); subst; clear H; clear H'
+    | H : int2Z _ = int2Z _ |- _ => rewrite ?H in *
+    | _ => try congruence; try omega; eauto
+end).
+
+
+  unfold insert. intros k v t n H. gen v; gen k.
+  induction H; try (cbn; eauto; fail); intros.
+    destruct
+    (IHis_redblack1 k v) as [n1 H1],
+    (IHis_redblack2 k v) as [n2 H2]. exists (S n). cbn. bd; constructor.
+        apply ins_is_redblack. assumption.
+        apply is_redblack_toblack. assumption.
+        apply is_redblack_toblack. assumption.
+        apply ins_is_redblack. assumption.
+    destruct
+    (IHis_redblack1 k v) as [n1 H1],
+    (IHis_redblack2 k v) as [n2 H2]. exists (S n). cbn.
+Admitted.
+
+End TREES.
+*)
